disk-betree/Graph.dfy
@@ -1,0 +1,9 @@
+abstract module Graph {
+  // Abstract features
+  type Reference(!new,==)
+  type Node(!new)
+  function Root() : Reference
+  function Successors(node: Node) : iset<Reference>
+
+  type Graph = imap<Reference, Node>
+}
